bin/gen/ExtractRomanWheel.v
@@ -13,6 +13,7 @@ Require Import TBGen.Util.OMap.
 Require Import TBGen.Bear.Sort.
 Require Import TBGen.Bear.BearGame.
 Require Import TBGen.Bear.RomanWheel.
+Require Import TBGen.Bear.RomanWheelSym.
 Require Import TBGen.TB.TB.
 
 Set Warnings "-extraction-default-directory".
