theory/Bear/RomanWheelSym.v
@@ -1,0 +1,240 @@
+Require Import List.
+Import ListNotations.
+
+Require Import PrimInt63.
+Require Import Uint63.
+Require Import ZArith.
+Require Import Lia.
+
+Require Import TBGen.Util.IntHash.
+Require Import TBGen.Bear.Graph.
+Require Import TBGen.Bear.BearGame.
+Require Import TBGen.TB.TB.
+Require Import TBGen.Bear.RomanWheel.
+
+Require Import TBGen.Bear.GroupAction.
+
+Definition Fin n : Type :=
+  { i : nat & i < n }.
+
+Definition val {n} (i : Fin n) : nat :=
+  projT1 i.
+
+(* technically doesn't need proof irrel. *)
+Lemma val_inj {n} (i j : Fin n) :
+  val i = val j -> i = j.
+Proof.
+  destruct i as [x x_pf].
+  destruct j as [y y_pf]; simpl.
+  intro pf; subst.
+  assert (x_pf = y_pf) by
+    apply ProofIrrelevance.proof_irrelevance.
+  subst; reflexivity.
+Qed.
+
+Definition Fin_zero {n} : Fin (S n).
+Proof.
+  exists 0; lia.
+Defined.
+
+Definition Fin_plus {n} : Fin n -> Fin n -> Fin n.
+Proof.
+  intros [x x_pf] [y y_pf].
+  exists ((x + y) mod n).
+  apply Nat.mod_upper_bound; lia.
+Defined.
+
+Lemma val_plus {n} (i j : Fin n) :
+  val (Fin_plus i j) = (val i + val j) mod n.
+Proof.
+  destruct i,j; simpl.
+  reflexivity.
+Qed.
+
+Definition Fin_inv {n} : Fin n -> Fin n.
+Proof.
+  intros [x x_pf].
+  exists (
+    match x with
+    | 0 => 0
+    | _ => n - x
+    end).
+  destruct x; lia.
+Defined.
+
+Lemma val_inv {n} (i : Fin n) :
+  val (Fin_inv i) =
+  match val i with
+  | 0 => 0
+  | _ => n - val i
+  end.
+Proof.
+  destruct i; reflexivity.
+Qed.
+
+Definition Z_8 : Group.
+Proof.
+  refine {|
+    carrier := Fin 8;
+    id := Fin_zero;
+    mult := Fin_plus;
+    inv := Fin_inv;
+    assoc := _;
+    id_left := _;
+    id_right := _;
+    inv_left := _;
+    inv_right := _;
+  |}.
+  - intros.
+    apply val_inj.
+    repeat rewrite val_plus.
+    rewrite Nat.Div0.add_mod_idemp_r.
+    rewrite Nat.Div0.add_mod_idemp_l.
+    now rewrite Nat.add_assoc.
+  - intros [x x_small].
+    apply val_inj.
+    rewrite val_plus.
+    simpl val.
+    rewrite Nat.mod_small; auto.
+  - intros [x x_small].
+    apply val_inj.
+    rewrite val_plus.
+    simpl val.
+    rewrite Nat.mod_small; auto; lia.
+  - intros [x x_small].
+    apply val_inj.
+    rewrite val_plus.
+    rewrite val_inv.
+    simpl val.
+    destruct x.
+    + reflexivity.
+    + assert (8 - S x + S x = 8) by lia.
+      rewrite H; reflexivity.
+  - intros [x x_small].
+    apply val_inj.
+    rewrite val_plus.
+    rewrite val_inv.
+    simpl val.
+    destruct x.
+    + reflexivity.
+    + assert (S x + (8 - S x) = 8) by lia.
+      rewrite H; reflexivity.
+Defined.
+
+Fixpoint rotate_spoke (n : nat) (s : Spoke) : Spoke :=
+  match n with
+  | 0 => s
+  | S m => clockwise (rotate_spoke m s)
+  end.
+
+Lemma rotate_spoke_plus (m n : nat) : forall (s : Spoke),
+  rotate_spoke (m + n) s =
+  rotate_spoke m (rotate_spoke n s).
+Proof.
+  induction m; intro.
+  - reflexivity.
+  - simpl.
+    now rewrite IHm.
+Qed.
+
+Lemma rotate_8 : forall s,
+  rotate_spoke 8 s = s.
+Proof.
+  intros []; reflexivity.
+Qed.
+
+Lemma rotate_mult_8 (n : nat) : forall (s : Spoke),
+  rotate_spoke (8 * n) s = s.
+Proof.
+  induction n; intro.
+  - reflexivity.
+  - rewrite <- mult_n_Sm.
+    rewrite rotate_spoke_plus.
+    rewrite rotate_8.
+    apply IHn.
+Qed.
+
+Lemma rotate_mod_8 (n : nat) : forall (s : Spoke),
+  rotate_spoke n s = rotate_spoke (n mod 8) s.
+Proof.
+  intro s.
+  rewrite (Nat.Div0.div_mod n 8) at 1.
+  rewrite rotate_spoke_plus.
+  now rewrite rotate_mult_8.
+Qed.
+
+Definition rotate_vert (n : nat) (v : RWVert) : RWVert :=
+  match v with
+  | Center => Center
+  | SpokeVert s l => SpokeVert (rotate_spoke n s) l
+  end.
+
+Global Instance RW_Z_8 : GroupAction RomanWheel Z_8.
+Proof.
+  refine {|
+    act := fun (x : carrier Z_8) (v : Vert RomanWheel) =>
+      rotate_vert (val x) v;
+    act_id := _;
+    act_comp := _;
+    act_edge := _;
+  |}.
+  - intros []; reflexivity.
+  - intros [] x y.
+    + reflexivity.
+    + simpl; f_equal.
+      rewrite val_plus.
+      rewrite <- rotate_mod_8.
+      now rewrite rotate_spoke_plus.
+  - intros x v v' pf.
+    destruct v.
+    + simpl rotate_vert.
+      apply cheat.
+    + apply cheat.
+Defined.
+
+Definition spoke_nat (s : Spoke) : nat :=
+  match s with
+  | S1 => 0
+  | S2 => 7
+  | S3 => 6
+  | S4 => 5
+  | S5 => 4
+  | S6 => 3
+  | S7 => 2
+  | S8 => 1
+  end.
+
+Lemma spoke_nat_small s : spoke_nat s < 8.
+Proof.
+  destruct s; simpl; lia.
+Qed.
+
+Definition spoke_Fin (s : Spoke) : Fin 8 :=
+  existT _ (spoke_nat s) (spoke_nat_small s).
+
+Definition compute_rotation (s : BG_State RomanWheel) : Fin 8.
+Proof.
+  destruct (bear s) eqn:?.
+  - destruct s; simpl in *.
+    destruct hunters.
+    + discriminate.
+    + destruct r.
+      * elim bear_not_hunter; now left.
+      * exact (spoke_Fin s).
+  - exact (spoke_Fin s0).
+Defined.
+
+Global Instance RW_OrbitSelector : OrbitSelector RomanWheel Z_8.
+Proof.
+  refine {|
+    select := fun s => BG_State_act (compute_rotation s) s
+  |}.
+  - intro s.
+    exists (compute_rotation s).
+    reflexivity.
+  - apply cheat.
+Defined.
+
+Definition RW_TB :=
+  Bear_TB RomanWheel Z_8.
+
